NTCB/ValidatorProof.v
@@ -1,0 +1,126 @@
+Require Import Lib.
+Require Import BinaryProps.
+Require Import List.
+Require Import LazyList.
+Require Import Semantics.
+Require Import SemanticsProp.
+Require Import NSet.
+Require Import BinaryProps.
+Require Import Recdef.
+Require Import Validator.
+
+
+Module ValProof (Import I : INSTRUCTION) (Import ISP: INSTRUCTION_SEMANTICS_PROP(I)).
+  Module Val := ValidatorCode(I).
+
+  Import Val.
+  Ltac fun_ind_validate_n_byte :=
+    match goal with
+      | |- context[ validate_n_byte ?n ?or ?a ?va ?tbca ?ll] =>
+        fun_ind_validate_n_byte_with
+          (validate_n_byte n or a va tbca ll)
+      | H : context[ validate_n_byte ?n ?or ?a ?va ?tbca ?ll] |- _ =>
+        fun_ind_validate_n_byte_with
+          (validate_n_byte n or a va tbca ll)
+    end.
+
+  Ltac fun_ind_validate_ll_with call :=
+    functional induction call;
+      [ fst_Case_tac "fun_ind_validate_ll 1"
+      | fst_Case_tac "fun_ind_validate_ll 2"
+      | fst_Case_tac "fun_ind_validate_ll 3"].
+
+  Ltac fun_ind_validate_ll :=
+    match goal with
+      | |- context[ validate_ll_list ?a ?va ?tbca ?ll] =>
+        fun_ind_validate_ll_with
+          (validate_ll_list a va tbca ll)
+      | H: context[ validate_ll_list ?a ?va ?tbca ?ll] |- _  =>
+        fun_ind_validate_ll_with
+          (validate_ll_list a va tbca ll)
+    end.
+
+
+  Lemma validate_n_byte_increase_valid_addresses:
+    forall (n: nat) (oreg: option register) (addr: N)
+    (valid_addresses to_be_checked_addresses: NSet) (ll: lazy_list byte)
+    valid_addresses' to_be_checked_addresses' ll',
+    validate_n_byte n oreg addr valid_addresses to_be_checked_addresses ll =
+    Some (valid_addresses', to_be_checked_addresses', ll') ->
+    Nincluded valid_addresses valid_addresses'.
+  Proof.
+    intros * VALIDATE.
+    fun_ind_validate_n_byte; clean; eauto with nset.
+  Qed.
+
+  Lemma validate_n_byte_increase_to_be_checked_addresses:
+    forall (n: nat) (oreg: option register) (addr: N)
+    (valid_addresses to_be_checked_addresses: NSet) (ll: lazy_list byte)
+    valid_addresses' to_be_checked_addresses' ll',
+    validate_n_byte n oreg addr valid_addresses to_be_checked_addresses ll =
+    Some (valid_addresses', to_be_checked_addresses', ll') ->
+    Nincluded to_be_checked_addresses to_be_checked_addresses'.
+  Proof.
+    intros * VALIDATE.
+    fun_ind_validate_n_byte; clean; eauto with nset.
+  Qed.
+
+  Lemma ll_safe_drop_plus: forall X n1 n2 (ll: lazy_list X),
+    ll_safe_drop (n1 + n2) ll = 
+    do ll' <- ll_safe_drop n1 ll;
+    ll_safe_drop n2 ll'.
+  Proof.
+    induction' n1 as [|n1]; intros; simpl in *; auto.
+    Case "S n1".
+      destruct' ll as [| x [ll1]]; auto.
+  Qed.
+      
+
+  Lemma validate_n_byte_drop_n:
+    forall (n: nat) (oreg: option register) (addr: N)
+    (valid_addresses to_be_checked_addresses: NSet) (ll: lazy_list byte)
+    valid_addresses' to_be_checked_addresses' ll',
+    validate_n_byte n oreg addr valid_addresses to_be_checked_addresses ll =
+    Some (valid_addresses', to_be_checked_addresses', ll') ->
+    ll_safe_drop n ll = Some ll'.
+  Proof.
+    intros * VALIDATE.
+    fun_ind_validate_n_byte; clean; eauto with nset;
+    apply safe_minus_correct in e3; subst;
+    rewrite ll_safe_drop_plus; rewrite e2; eauto.
+  Qed.
+  Local Hint Resolve validate_n_byte_drop_n validate_n_byte_increase_to_be_checked_addresses
+    validate_n_byte_increase_valid_addresses.
+
+  Lemma validate_ll_list_increase_valid_addresses:
+    forall (addr: N)
+    (valid_addresses to_be_checked_addresses: NSet) (ll: lazy_list byte)
+    valid_addresses' to_be_checked_addresses',
+    validate_ll_list addr valid_addresses to_be_checked_addresses ll =
+    Some (valid_addresses', to_be_checked_addresses') ->
+    Nincluded valid_addresses valid_addresses'.
+  Proof.
+    intros * VALIDATE.
+    fun_ind_validate_ll; clean; eauto with nset.
+  Qed.
+
+  Lemma validate_ll_list_increase_to_be_checked_addresses:
+    forall (addr: N)
+    (valid_addresses to_be_checked_addresses: NSet) (ll: lazy_list byte)
+    valid_addresses' to_be_checked_addresses',
+    validate_ll_list addr valid_addresses to_be_checked_addresses ll =
+    Some (valid_addresses', to_be_checked_addresses') ->
+    Nincluded to_be_checked_addresses to_be_checked_addresses'.
+  Proof.
+    intros * VALIDATE.
+    fun_ind_validate_ll; clean; eauto with nset.
+  Qed.
+
+  Local Hint Resolve validate_ll_list_increase_to_be_checked_addresses 
+    validate_ll_list_increase_valid_addresses.
+
+
+
+
+
+End ValProof.
